lean/lakefile.lean
@@ -1,6 +1,8 @@
 import Lake
 open Lake DSL
 
+require "leanprover-community" / "mathlib" @ git "v4.12.0"
+
 package cta where
   leanOptions := #[
     ⟨`pp.unicode.fun, true⟩
